rebase and fix problems caused by new machine constants

spec/design/ARM/ArchVSpace_H.thy
@@ -22,9 +22,6 @@ begin
 defs vptrFromPPtr_def:
 "vptrFromPPtr ptr \<equiv> returnOk $ ptr + 0x20000000"
 
-defs kernelBase_def:
-"kernelBase \<equiv> VPtr 0xf0000000"
-
 defs globalsBase_def:
 "globalsBase \<equiv> VPtr 0xffffc000"
 
