proof/invariant-abstract/PDPTEntries_AI.thy
@@ -576,11 +576,11 @@ lemma copy_global_mappings_valid_pdpt_objs[wp]:
     apply (clarsimp split:if_splits)
      apply (simp add:kernel_base_shift_cast_le)
      apply (simp add:kernel_base_def)
-     apply (cut_tac y1 = xb and x1 = "0xF00::12 word" in ucast_le_migrate[THEN iffD1,rotated -1])
+     apply (cut_tac y1 = xb and x1 = "0xE00::12 word" in ucast_le_migrate[THEN iffD1,rotated -1])
         apply simp
        apply (simp add:word_size le_less_trans)
       apply (simp add:word_size)
-     apply (drule aligned_le_sharp[where n = 4 and a = "0xF00::12 word"])
+     apply (drule aligned_le_sharp[where n = 4 and a = "0xE00::12 word"])
       apply (simp add:kernel_base_def is_aligned_def)
      apply (erule order_trans)
      apply (erule subst)
