spec/machine/ARM/Platform.thy
@@ -43,11 +43,16 @@ definition
 
 definition
   kernelBase_addr :: word32 where
-  "kernelBase_addr \<equiv> 0xf0000000"
+  "kernelBase_addr \<equiv> 0xe0000000"
+
+(* Arch specific kernel base address used for haskell spec *)
+definition
+  kernelBase :: word32 where
+  "kernelBase \<equiv> 0xe0000000"
 
 definition
   physBase :: word32 where
-  "physBase \<equiv> 0x80000000"
+  "physBase \<equiv> 0x10000000"
 
 definition
   physMappingOffset :: word32 where
@@ -67,6 +72,6 @@ definition
 
 definition
   maxIRQ :: "irq" where
-  "maxIRQ \<equiv> 63"
+  "maxIRQ \<equiv> 0x9F"
 
 end
